<?xml version="1.0"?>
<rdf:RDF xmlns="http://www.ease-crc.org/ont/EASE-WF.owl#"
     xml:base="http://www.ease-crc.org/ont/EASE-WF.owl"
     xmlns:rdf="http://www.w3.org/1999/02/22-rdf-syntax-ns#"
     xmlns:owl="http://www.w3.org/2002/07/owl#"
     xmlns:xml="http://www.w3.org/XML/1998/namespace"
     xmlns:swrl="http://www.w3.org/2003/11/swrl#"
     xmlns:xsd="http://www.w3.org/2001/XMLSchema#"
     xmlns:knowrob="http://knowrob.org/kb/knowrob.owl#"
     xmlns:rdfs="http://www.w3.org/2000/01/rdf-schema#"
     xmlns:EASE="http://www.ease-crc.org/ont/EASE.owl#"
     xmlns:ease_wf="http://www.ease-crc.org/ont/EASE-WF.owl#">
    <owl:Ontology rdf:about="http://www.ease-crc.org/ont/EASE-WF.owl">
        <owl:imports rdf:resource="package://ease_ontologies/owl/EASE.owl"/>
        <owl:imports rdf:resource="http://www.ontologydesignpatterns.org/ont/dul/DUL.owl"/>
        <owl:imports rdf:resource="http://www.ontologydesignpatterns.org/ont/dul/IOLite.owl"/>
    </owl:Ontology>
    


    <!-- 
    ///////////////////////////////////////////////////////////////////////////////////////
    //
    // Object Properties
    //
    ///////////////////////////////////////////////////////////////////////////////////////
     -->

    


    <!-- http://www.ease-crc.org/ont/EASE-WF.owl#definesInput -->

    <owl:ObjectProperty rdf:about="http://www.ease-crc.org/ont/EASE-WF.owl#definesInput">
        <rdfs:subPropertyOf rdf:resource="http://www.ease-crc.org/ont/EASE-WF.owl#definesParticipant"/>
        <rdfs:domain rdf:resource="http://www.ontologydesignpatterns.org/ont/dul/DUL.owl#Description"/>
        <rdfs:range>
            <owl:Class>
                <owl:unionOf rdf:parseType="Collection">
                    <rdf:Description rdf:about="http://www.ontologydesignpatterns.org/ont/dul/DUL.owl#Parameter"/>
                    <rdf:Description rdf:about="http://www.ontologydesignpatterns.org/ont/dul/DUL.owl#Role"/>
                </owl:unionOf>
            </owl:Class>
        </rdfs:range>
        <rdfs:comment>The defined participant is an &quot;input&quot;: 

- some object existing at the beginning of a Task&apos;s execution, and that will be acted on during the execution of the task;
- some region/value which informs the way in which the Task will be executed.</rdfs:comment>
    </owl:ObjectProperty>
    


    <!-- http://www.ease-crc.org/ont/EASE-WF.owl#definesOutput -->

    <owl:ObjectProperty rdf:about="http://www.ease-crc.org/ont/EASE-WF.owl#definesOutput">
        <rdfs:subPropertyOf rdf:resource="http://www.ease-crc.org/ont/EASE-WF.owl#definesParticipant"/>
        <rdfs:domain rdf:resource="http://www.ontologydesignpatterns.org/ont/dul/DUL.owl#Description"/>
        <rdfs:range>
            <owl:Class>
                <owl:unionOf rdf:parseType="Collection">
                    <rdf:Description rdf:about="http://www.ontologydesignpatterns.org/ont/dul/DUL.owl#Parameter"/>
                    <rdf:Description rdf:about="http://www.ontologydesignpatterns.org/ont/dul/DUL.owl#Role"/>
                </owl:unionOf>
            </owl:Class>
        </rdfs:range>
        <rdfs:comment>Defines an &quot;output&quot; participant:

- an Entity (Object or state of affairs) that exists as a result of the execution of a Task;
- a Region/value that has been demarcated/computed as a result of the execution of a Task.</rdfs:comment>
    </owl:ObjectProperty>
    


    <!-- http://www.ease-crc.org/ont/EASE-WF.owl#definesParticipant -->

    <owl:ObjectProperty rdf:about="http://www.ease-crc.org/ont/EASE-WF.owl#definesParticipant">
        <rdfs:subPropertyOf rdf:resource="http://www.ontologydesignpatterns.org/ont/dul/DUL.owl#defines"/>
        <rdfs:domain rdf:resource="http://www.ontologydesignpatterns.org/ont/dul/DUL.owl#Description"/>
        <rdfs:range rdf:resource="http://www.ontologydesignpatterns.org/ont/dul/DUL.owl#Concept"/>
        <rdfs:comment>A Description definesParticipant a Concept to classify participants in Events associated to that Description.

The prototypical example is a Task, which is a concept to classify Actions (a form of Event). A Task may define several Roles, with which to classify participants in the event of that Task&apos;s execution.</rdfs:comment>
    </owl:ObjectProperty>
    


    <!-- http://www.ease-crc.org/ont/EASE-WF.owl#hasBinding -->

    <owl:ObjectProperty rdf:about="http://www.ease-crc.org/ont/EASE-WF.owl#hasBinding">
        <rdfs:subPropertyOf rdf:resource="http://www.ontologydesignpatterns.org/ont/dul/DUL.owl#hasPart"/>
        <rdfs:domain rdf:resource="http://www.ontologydesignpatterns.org/ont/dul/DUL.owl#Description"/>
        <rdfs:range rdf:resource="http://www.ease-crc.org/ont/EASE-WF.owl#Binding"/>
        <rdfs:comment>Asserts that in a context described by Description, a Binding relation holds.</rdfs:comment>
    </owl:ObjectProperty>
    


    <!-- http://www.ease-crc.org/ont/EASE-WF.owl#hasBindingFiller -->

    <owl:ObjectProperty rdf:about="http://www.ease-crc.org/ont/EASE-WF.owl#hasBindingFiller">
        <rdfs:subPropertyOf rdf:resource="http://www.ontologydesignpatterns.org/ont/dul/DUL.owl#describes"/>
        <rdfs:domain rdf:resource="http://www.ease-crc.org/ont/EASE-WF.owl#Binding"/>
        <rdfs:range rdf:resource="http://www.ontologydesignpatterns.org/ont/dul/DUL.owl#Entity"/>
        <rdfs:comment>Indicates that an Entity is described by a Binding, in that it is associated with the Role/Parameter that the Binding binds it to. The Binding is only valid in some descriptive context such as a Workflow or Narrative.

Note, the filler can be a Role/Parameter as well, and there are two distinct interpretations, depending on whether the Binding is a RoleRoleBinding or a RoleFillerBinding. See the comments on Binding for more details.

Only RoleFillerBindings can have general Entities as fillers. RoleRoleBindings can only connect to Roles or Parameters via this property.</rdfs:comment>
    </owl:ObjectProperty>
    


    <!-- http://www.ease-crc.org/ont/EASE-WF.owl#hasBindingRole -->

    <owl:ObjectProperty rdf:about="http://www.ease-crc.org/ont/EASE-WF.owl#hasBindingRole">
        <rdfs:subPropertyOf rdf:resource="http://www.ontologydesignpatterns.org/ont/dul/DUL.owl#hasPart"/>
        <rdfs:domain rdf:resource="http://www.ease-crc.org/ont/EASE-WF.owl#Binding"/>
        <rdfs:range>
            <owl:Class>
                <owl:unionOf rdf:parseType="Collection">
                    <rdf:Description rdf:about="http://www.ontologydesignpatterns.org/ont/dul/DUL.owl#Parameter"/>
                    <rdf:Description rdf:about="http://www.ontologydesignpatterns.org/ont/dul/DUL.owl#Role"/>
                </owl:unionOf>
            </owl:Class>
        </rdfs:range>
        <rdfs:comment>Indicates that a Role/Parameter is going to be associated to some filler, or other Role/Parameter, by a Binding. The Binding is only valid in some descriptive context such as a Narrative or Workflow.</rdfs:comment>
    </owl:ObjectProperty>
    


    <!-- http://www.ease-crc.org/ont/EASE-WF.owl#hasPredecessorTask -->

    <owl:ObjectProperty rdf:about="http://www.ease-crc.org/ont/EASE-WF.owl#hasPredecessorTask">
        <rdfs:subPropertyOf rdf:resource="http://www.ease-crc.org/ont/EASE-WF.owl#hasTask"/>
        <rdfs:domain rdf:resource="http://www.ease-crc.org/ont/EASE-WF.owl#Succedence"/>
        <rdfs:range rdf:resource="http://www.ontologydesignpatterns.org/ont/dul/DUL.owl#Task"/>
        <rdfs:comment>Indicates that a Task is the predecessor in a Succedence Relation; that is, this is the task to execute first.</rdfs:comment>
    </owl:ObjectProperty>
    


    <!-- http://www.ease-crc.org/ont/EASE-WF.owl#hasSuccedence -->

    <owl:ObjectProperty rdf:about="http://www.ease-crc.org/ont/EASE-WF.owl#hasSuccedence">
        <rdfs:subPropertyOf rdf:resource="http://www.ontologydesignpatterns.org/ont/dul/DUL.owl#hasPart"/>
        <rdfs:domain rdf:resource="http://www.ontologydesignpatterns.org/ont/dul/DUL.owl#Workflow"/>
        <rdfs:range rdf:resource="http://www.ease-crc.org/ont/EASE-WF.owl#Succedence"/>
    </owl:ObjectProperty>
    


    <!-- http://www.ease-crc.org/ont/EASE-WF.owl#hasSuccessorTask -->

    <owl:ObjectProperty rdf:about="http://www.ease-crc.org/ont/EASE-WF.owl#hasSuccessorTask">
        <rdfs:subPropertyOf rdf:resource="http://www.ease-crc.org/ont/EASE-WF.owl#hasTask"/>
        <rdfs:domain rdf:resource="http://www.ease-crc.org/ont/EASE-WF.owl#Succedence"/>
        <rdfs:range rdf:resource="http://www.ontologydesignpatterns.org/ont/dul/DUL.owl#Task"/>
        <rdfs:comment>Indicates that a Task is the successor in a Succedence Relation: that is, it is the Task to execute last.</rdfs:comment>
    </owl:ObjectProperty>
    


    <!-- http://www.ease-crc.org/ont/EASE-WF.owl#hasTask -->

    <owl:ObjectProperty rdf:about="http://www.ease-crc.org/ont/EASE-WF.owl#hasTask">
        <rdfs:subPropertyOf rdf:resource="http://www.ontologydesignpatterns.org/ont/dul/DUL.owl#hasPart"/>
        <rdfs:domain>
            <owl:Class>
                <owl:unionOf rdf:parseType="Collection">
                    <rdf:Description rdf:about="http://www.ontologydesignpatterns.org/ont/dul/DUL.owl#Relation"/>
                    <rdf:Description rdf:about="http://www.ontologydesignpatterns.org/ont/dul/DUL.owl#Workflow"/>
                </owl:unionOf>
            </owl:Class>
        </rdfs:domain>
        <rdfs:range rdf:resource="http://www.ontologydesignpatterns.org/ont/dul/DUL.owl#Task"/>
        <rdfs:comment>A relation to indicate that a Task is part of a Workflow or ordering Relation: that is, the task may be executed during the execution of the Workflow, or there exists some Relation between the Tasks that informs how their executions are to be located in time.</rdfs:comment>
    </owl:ObjectProperty>
    


    <!-- http://www.ontologydesignpatterns.org/ont/dul/DUL.owl#defines -->

    <owl:ObjectProperty rdf:about="http://www.ontologydesignpatterns.org/ont/dul/DUL.owl#defines"/>
    


    <!-- http://www.ontologydesignpatterns.org/ont/dul/DUL.owl#describes -->

    <owl:ObjectProperty rdf:about="http://www.ontologydesignpatterns.org/ont/dul/DUL.owl#describes"/>
    


    <!-- http://www.ontologydesignpatterns.org/ont/dul/DUL.owl#hasPart -->

    <owl:ObjectProperty rdf:about="http://www.ontologydesignpatterns.org/ont/dul/DUL.owl#hasPart"/>
    


    <!-- 
    ///////////////////////////////////////////////////////////////////////////////////////
    //
    // Classes
    //
    ///////////////////////////////////////////////////////////////////////////////////////
     -->

    


    <!-- http://www.ease-crc.org/ont/EASE-WF.owl#Binding -->

    <owl:Class rdf:about="http://www.ease-crc.org/ont/EASE-WF.owl#Binding">
        <rdfs:subClassOf rdf:resource="http://www.ontologydesignpatterns.org/ont/dul/DUL.owl#Relation"/>
        <rdfs:subClassOf>
            <owl:Class>
                <owl:unionOf rdf:parseType="Collection">
                    <rdf:Description rdf:about="http://www.ease-crc.org/ont/EASE-WF.owl#CounterfactualBinding"/>
                    <rdf:Description rdf:about="http://www.ease-crc.org/ont/EASE-WF.owl#FactualBinding"/>
                </owl:unionOf>
            </owl:Class>
        </rdfs:subClassOf>
        <rdfs:subClassOf>
            <owl:Class>
                <owl:unionOf rdf:parseType="Collection">
                    <rdf:Description rdf:about="http://www.ease-crc.org/ont/EASE-WF.owl#RoleFillerBinding"/>
                    <rdf:Description rdf:about="http://www.ease-crc.org/ont/EASE-WF.owl#RoleRoleBinding"/>
                </owl:unionOf>
            </owl:Class>
        </rdfs:subClassOf>
        <rdfs:subClassOf>
            <owl:Restriction>
                <owl:onProperty>
                    <rdf:Description>
                        <owl:inverseOf rdf:resource="http://www.ease-crc.org/ont/EASE-WF.owl#hasBinding"/>
                    </rdf:Description>
                </owl:onProperty>
                <owl:someValuesFrom rdf:resource="http://www.ontologydesignpatterns.org/ont/dul/DUL.owl#Description"/>
            </owl:Restriction>
        </rdfs:subClassOf>
        <rdfs:subClassOf>
            <owl:Restriction>
                <owl:onProperty rdf:resource="http://www.ease-crc.org/ont/EASE-WF.owl#hasBindingFiller"/>
                <owl:qualifiedCardinality rdf:datatype="http://www.w3.org/2001/XMLSchema#nonNegativeInteger">1</owl:qualifiedCardinality>
                <owl:onClass rdf:resource="http://www.ontologydesignpatterns.org/ont/dul/DUL.owl#Entity"/>
            </owl:Restriction>
        </rdfs:subClassOf>
        <rdfs:subClassOf>
            <owl:Restriction>
                <owl:onProperty rdf:resource="http://www.ease-crc.org/ont/EASE-WF.owl#hasBindingRole"/>
                <owl:qualifiedCardinality rdf:datatype="http://www.w3.org/2001/XMLSchema#nonNegativeInteger">1</owl:qualifiedCardinality>
                <owl:onClass>
                    <owl:Class>
                        <owl:unionOf rdf:parseType="Collection">
                            <rdf:Description rdf:about="http://www.ontologydesignpatterns.org/ont/dul/DUL.owl#Parameter"/>
                            <rdf:Description rdf:about="http://www.ontologydesignpatterns.org/ont/dul/DUL.owl#Role"/>
                        </owl:unionOf>
                    </owl:Class>
                </owl:onClass>
            </owl:Restriction>
        </rdfs:subClassOf>
        <rdfs:comment>A Relation between Roles/Parameters and their fillers that holds in a particular descriptive context, such as a Workflow or Narrative.

It covers two conceptually related, but somewhat ontologically distinct situations:

-- a binding between two Roles, or two Parameters, with the meaning that in the particular descriptive context where the Binding holds, a filler for one Role/Parameter is also a filler for the other
-- a binding between a Role/Parameter and an Entity able to fill that Role/Parameter, with the meaning that in the particular descriptive context where the Binding holds, the Entity fills the Role/Parameter.

Note: in the second case, the Entity filling the Role/Parameter may be a Role or Parameter itself. This however does NOT reduce to the first case. Consider these examples:

-- (first situation) The accountant is also the lawyer. In this case, there are two roles, and there is a person filling both of them. This is a factual, role-role binding.
-- (second situation, linking to a generic Entity) The accountant is Bob. In this case, there is a factual, role-filler binding asserting who fills the accountant role.
-- (second situation, linking to a role) The newly opened job is accountant. In this case, there is a factual, role-filler binding asserting that some role is filled by another, without making any assertion about the filler of this second role. It is not known, and not important, whether an accountant exists at this time.

There is a further, orthogonal distinction made between:
-- factual: the Binding is asserted to hold in the descriptive context
-- counterfactual: the Binding is used to express conditions in the descriptive context. A counterfactual Binding is not meant as an assertion that the Binding actually holds.</rdfs:comment>
    </owl:Class>
    


    <!-- http://www.ease-crc.org/ont/EASE-WF.owl#ConditionalSuccedence -->

    <owl:Class rdf:about="http://www.ease-crc.org/ont/EASE-WF.owl#ConditionalSuccedence">
        <rdfs:subClassOf rdf:resource="http://www.ease-crc.org/ont/EASE-WF.owl#Succedence"/>
        <rdfs:subClassOf>
            <owl:Restriction>
                <owl:onProperty rdf:resource="http://www.ease-crc.org/ont/EASE-WF.owl#hasBinding"/>
                <owl:allValuesFrom rdf:resource="http://www.ease-crc.org/ont/EASE-WF.owl#CounterfactualBinding"/>
            </owl:Restriction>
        </rdfs:subClassOf>
        <rdfs:comment>A relation that holds between two RobotTasks that belong to the same RobotWorkflow, and which means that, if a condition is met, the successor task is to be executed after the predecessor task completes.

The condition is a conjunction of CounterfactualBindings. These bindings may be RoleRoleBindings (meaning, test whether the fillers for these Roles/Parameters are the same) or RoleFillerBindings (meaning, test whether the filler of the Role unifies with the candidate Entity).

An empty conjunction of CounterfactualBindings is assumed to be True.</rdfs:comment>
        <rdfs:comment>Note: in RobotWorkflows, Tasks typically may have several possible successors, to be selected based on condition-testing.</rdfs:comment>
    </owl:Class>
    


    <!-- http://www.ease-crc.org/ont/EASE-WF.owl#CounterfactualBinding -->

    <owl:Class rdf:about="http://www.ease-crc.org/ont/EASE-WF.owl#CounterfactualBinding">
        <rdfs:subClassOf rdf:resource="http://www.ease-crc.org/ont/EASE-WF.owl#Binding"/>
        <owl:disjointWith rdf:resource="http://www.ease-crc.org/ont/EASE-WF.owl#FactualBinding"/>
        <rdfs:comment>CounterfactualBindings are used to express conditions:

-- that two roles share a filler (RoleRoleBindings);
-- that the filler of a role is a particular entity (RoleFillerBindings). This is typically the case when the filler of the role may be one of a few constants, as is the case with the execution status of a robot task.

TODO: for the robot workflows we are likely to need at the start, testing equality of fillers is enough. In the future, we may want to replace that with unifiability of fillers.</rdfs:comment>
    </owl:Class>
    


    <!-- http://www.ease-crc.org/ont/EASE-WF.owl#EntryRobotWorkflow -->

    <owl:Class rdf:about="http://www.ease-crc.org/ont/EASE-WF.owl#EntryRobotWorkflow">
        <rdfs:subClassOf rdf:resource="http://www.ease-crc.org/ont/EASE-WF.owl#RobotTask"/>
        <rdfs:subClassOf>
            <owl:Restriction>
                <owl:onProperty rdf:resource="http://www.ease-crc.org/ont/EASE-WF.owl#definesOutput"/>
                <owl:qualifiedCardinality rdf:datatype="http://www.w3.org/2001/XMLSchema#nonNegativeInteger">0</owl:qualifiedCardinality>
                <owl:onClass rdf:resource="http://www.ontologydesignpatterns.org/ont/dul/DUL.owl#Entity"/>
            </owl:Restriction>
        </rdfs:subClassOf>
        <owl:disjointWith rdf:resource="http://www.ease-crc.org/ont/EASE-WF.owl#ExitRobotWorkflow"/>
        <rdfs:comment>Note: equality constraints between parameter sets for Entry/Exit points and the RobotTask defined by a RobotWorkflow might suggest that the RobotTask defined by the workflow can be used as an entry/exit point.

This however is not the case, as these tasks have different meanings for the KnowRob workflow interpreter.

-- work-flow defined task: any general purpose task, such as some robot behavior, described by a workflow. Encountering such a task during a run of the interpreter will evoke the defining workflow.
-- entry point task: bind roles and parameters in the workflow to values obtained from the evoker of the workflow
-- exit point task: bind roles and parameters in the workflow to outputs, and return control to the workflow&apos;s evoker.</rdfs:comment>
        <rdfs:comment>The first Task in a RobotWorkflow, which is simply to receive the inputs and bind them to the appropriate roles defined in the workflow.

A RobotWorkflow has only 1 entry point.

This task has no outputs.</rdfs:comment>
        <rdfs:comment>WARNING: the following constraint was not modelled in the Tbox, but it is expected that RobotWorkflows will implement it.

The EntryRobotWorkflow should have the same inputs as the RobotTask defined by the RobotWorkflow.</rdfs:comment>
    </owl:Class>
    


    <!-- http://www.ease-crc.org/ont/EASE-WF.owl#ExitRobotWorkflow -->

    <owl:Class rdf:about="http://www.ease-crc.org/ont/EASE-WF.owl#ExitRobotWorkflow">
        <rdfs:subClassOf rdf:resource="http://www.ease-crc.org/ont/EASE-WF.owl#RobotTask"/>
        <rdfs:subClassOf>
            <owl:Restriction>
                <owl:onProperty rdf:resource="http://www.ease-crc.org/ont/EASE-WF.owl#definesInput"/>
                <owl:qualifiedCardinality rdf:datatype="http://www.w3.org/2001/XMLSchema#nonNegativeInteger">0</owl:qualifiedCardinality>
                <owl:onClass rdf:resource="http://www.ontologydesignpatterns.org/ont/dul/DUL.owl#Entity"/>
            </owl:Restriction>
        </rdfs:subClassOf>
        <rdfs:comment>A final Task in a RobotWorkflow, which is simply to return some information as a &quot;result&quot; of the workflow&apos;s execution.

This task only uses outputs. The values for the outputs are calculated by the KnowRob workflow interpreter based on the Bindings between roles that exist in the workflow.</rdfs:comment>
    </owl:Class>
    


    <!-- http://www.ease-crc.org/ont/EASE-WF.owl#FactualBinding -->

    <owl:Class rdf:about="http://www.ease-crc.org/ont/EASE-WF.owl#FactualBinding">
        <rdfs:subClassOf rdf:resource="http://www.ease-crc.org/ont/EASE-WF.owl#Binding"/>
        <rdfs:comment>FactualBindings are used in a workflow to assert that:

-- task- or workflow-defined roles share fillers (RoleRoleBindings). Example, the instrument of a cutting task may be the actee of a grasping task;
-- task- or workflow-defined roles are filled by a particular entity (RoleFillerBindings). This is typically the case when roles, and especially parameters, can be assigned to constants. Example, the waiting time to cook soft eggs is 3 minutes.</rdfs:comment>
    </owl:Class>
    


    <!-- http://www.ease-crc.org/ont/EASE-WF.owl#RobotTask -->

    <owl:Class rdf:about="http://www.ease-crc.org/ont/EASE-WF.owl#RobotTask">
        <rdfs:subClassOf rdf:resource="http://www.ontologydesignpatterns.org/ont/dul/DUL.owl#Task"/>
        <rdfs:subClassOf>
            <owl:Restriction>
                <owl:onProperty rdf:resource="http://www.ease-crc.org/ont/EASE-WF.owl#definesInput"/>
                <owl:allValuesFrom>
                    <owl:Class>
                        <owl:unionOf rdf:parseType="Collection">
                            <rdf:Description rdf:about="http://www.ontologydesignpatterns.org/ont/dul/DUL.owl#Parameter"/>
                            <rdf:Description rdf:about="http://www.ontologydesignpatterns.org/ont/dul/DUL.owl#Role"/>
                        </owl:unionOf>
                    </owl:Class>
                </owl:allValuesFrom>
            </owl:Restriction>
        </rdfs:subClassOf>
        <rdfs:subClassOf>
            <owl:Restriction>
                <owl:onProperty rdf:resource="http://www.ease-crc.org/ont/EASE-WF.owl#definesOutput"/>
                <owl:allValuesFrom>
                    <owl:Class>
                        <owl:unionOf rdf:parseType="Collection">
                            <rdf:Description rdf:about="http://www.ontologydesignpatterns.org/ont/dul/DUL.owl#Parameter"/>
                            <rdf:Description rdf:about="http://www.ontologydesignpatterns.org/ont/dul/DUL.owl#Role"/>
                        </owl:unionOf>
                    </owl:Class>
                </owl:allValuesFrom>
            </owl:Restriction>
        </rdfs:subClassOf>
        <rdfs:comment>A Task to be interpreted by the KnowRob Workflow interpreter.

Usually, has a non-empty set of input (Role or Parameter)s, and a non-empty set of output (Role or Parameter)s-- however, eiter or both of these sets may be empty in the case of tasks with trivial input/outputs.</rdfs:comment>
    </owl:Class>
    


    <!-- http://www.ease-crc.org/ont/EASE-WF.owl#RobotWorkflow -->

    <owl:Class rdf:about="http://www.ease-crc.org/ont/EASE-WF.owl#RobotWorkflow">
        <rdfs:subClassOf rdf:resource="http://www.ontologydesignpatterns.org/ont/dul/DUL.owl#Workflow"/>
        <rdfs:subClassOf>
            <owl:Restriction>
                <owl:onProperty rdf:resource="http://www.ease-crc.org/ont/EASE-WF.owl#hasTask"/>
                <owl:someValuesFrom rdf:resource="http://www.ease-crc.org/ont/EASE-WF.owl#ExitRobotWorkflow"/>
            </owl:Restriction>
        </rdfs:subClassOf>
        <rdfs:subClassOf>
            <owl:Restriction>
                <owl:onProperty rdf:resource="http://www.ease-crc.org/ont/EASE-WF.owl#hasBinding"/>
                <owl:allValuesFrom rdf:resource="http://www.ease-crc.org/ont/EASE-WF.owl#FactualBinding"/>
            </owl:Restriction>
        </rdfs:subClassOf>
        <rdfs:subClassOf>
            <owl:Restriction>
                <owl:onProperty rdf:resource="http://www.ease-crc.org/ont/EASE-WF.owl#hasSuccedence"/>
                <owl:allValuesFrom rdf:resource="http://www.ease-crc.org/ont/EASE-WF.owl#ConditionalSuccedence"/>
            </owl:Restriction>
        </rdfs:subClassOf>
        <rdfs:subClassOf>
            <owl:Restriction>
                <owl:onProperty rdf:resource="http://www.ease-crc.org/ont/EASE-WF.owl#hasTask"/>
                <owl:allValuesFrom rdf:resource="http://www.ease-crc.org/ont/EASE-WF.owl#RobotTask"/>
            </owl:Restriction>
        </rdfs:subClassOf>
        <rdfs:subClassOf>
            <owl:Restriction>
                <owl:onProperty rdf:resource="http://www.ease-crc.org/ont/EASE-WF.owl#hasTask"/>
                <owl:qualifiedCardinality rdf:datatype="http://www.w3.org/2001/XMLSchema#nonNegativeInteger">1</owl:qualifiedCardinality>
                <owl:onClass rdf:resource="http://www.ease-crc.org/ont/EASE-WF.owl#EntryRobotWorkflow"/>
            </owl:Restriction>
        </rdfs:subClassOf>
        <rdfs:subClassOf>
            <owl:Restriction>
                <owl:onProperty rdf:resource="http://www.ontologydesignpatterns.org/ont/dul/DUL.owl#defines"/>
                <owl:qualifiedCardinality rdf:datatype="http://www.w3.org/2001/XMLSchema#nonNegativeInteger">1</owl:qualifiedCardinality>
                <owl:onClass rdf:resource="http://www.ease-crc.org/ont/EASE-WF.owl#RobotTask"/>
            </owl:Restriction>
        </rdfs:subClassOf>
        <rdfs:comment>A natural exit of a RobotWorkflow is the arrival at an ExitRobotWorkflow task.

A premature exit will however happen when a RobotTask is completed, which is not an ExitRobotWorkflow, and which has no triggerable ConditionalSuccedence relations for which it is the predecessor task.

This situation can occur when

-- the RobotTask in question is not a predecessor task for any ConditionalSuccedence in the workflow;
-- none of the ConditionalSuccedence relations that have the task as predecessor can fire, because neither of their conditions are met.

Both of these situations are errors: they signal that the workflow is incompletely described.</rdfs:comment>
        <rdfs:comment>A workflow meant to guide the action of a robot agent and interpreted by the KnowRob workflow interpreter.

It defines exactly one RobotTask, but may contain several RobotTasks linked by ConditionalSuccedence relations.

It has at most one entry point, which is the first RobotTask to execute when enacting the Workflow. If no first task is present, then the Workflow is empty.

It may have several exit points. When an exit point is reached, the Workflow execution has completed. They result in a termination of the workflow, and a return to its invoker, with a special error status and a record of the output of the last task.</rdfs:comment>
        <rdfs:comment>WARNING: not all constraints are easy to enforce in OWL Tboxes; in particular, the following constraints have not been modelled in the Tbox. It is required however that RobotWorkflows obey them.

-- the input parameters of the RobotTask defined by the RobotWorkflow are exactly the same as the input parameters of the EntryRobotWorkflow belonging to the RobotWorkflow;
-- the output parameters of the RobotTask defined by the RobotWorkflow are exactly the same as the output parameters defined by every ExitRobotWorkflow belonging to the RobotWorkflow.</rdfs:comment>
    </owl:Class>
    


    <!-- http://www.ease-crc.org/ont/EASE-WF.owl#RoleFillerBinding -->

    <owl:Class rdf:about="http://www.ease-crc.org/ont/EASE-WF.owl#RoleFillerBinding">
        <rdfs:subClassOf rdf:resource="http://www.ease-crc.org/ont/EASE-WF.owl#Binding"/>
        <owl:disjointWith rdf:resource="http://www.ease-crc.org/ont/EASE-WF.owl#RoleRoleBinding"/>
    </owl:Class>
    


    <!-- http://www.ease-crc.org/ont/EASE-WF.owl#RoleRoleBinding -->

    <owl:Class rdf:about="http://www.ease-crc.org/ont/EASE-WF.owl#RoleRoleBinding">
        <rdfs:subClassOf rdf:resource="http://www.ease-crc.org/ont/EASE-WF.owl#Binding"/>
        <rdfs:subClassOf>
            <owl:Restriction>
                <owl:onProperty rdf:resource="http://www.ease-crc.org/ont/EASE-WF.owl#hasBindingFiller"/>
                <owl:allValuesFrom>
                    <owl:Class>
                        <owl:unionOf rdf:parseType="Collection">
                            <rdf:Description rdf:about="http://www.ontologydesignpatterns.org/ont/dul/DUL.owl#Parameter"/>
                            <rdf:Description rdf:about="http://www.ontologydesignpatterns.org/ont/dul/DUL.owl#Role"/>
                        </owl:unionOf>
                    </owl:Class>
                </owl:allValuesFrom>
            </owl:Restriction>
        </rdfs:subClassOf>
    </owl:Class>
    


    <!-- http://www.ease-crc.org/ont/EASE-WF.owl#Succedence -->

    <owl:Class rdf:about="http://www.ease-crc.org/ont/EASE-WF.owl#Succedence">
        <rdfs:subClassOf rdf:resource="http://www.ontologydesignpatterns.org/ont/dul/DUL.owl#Relation"/>
        <rdfs:subClassOf>
            <owl:Restriction>
                <owl:onProperty>
                    <rdf:Description>
                        <owl:inverseOf rdf:resource="http://www.ease-crc.org/ont/EASE-WF.owl#hasSuccedence"/>
                    </rdf:Description>
                </owl:onProperty>
                <owl:someValuesFrom rdf:resource="http://www.ontologydesignpatterns.org/ont/dul/DUL.owl#Description"/>
            </owl:Restriction>
        </rdfs:subClassOf>
        <rdfs:subClassOf>
            <owl:Restriction>
                <owl:onProperty rdf:resource="http://www.ease-crc.org/ont/EASE-WF.owl#hasPredecessorTask"/>
                <owl:qualifiedCardinality rdf:datatype="http://www.w3.org/2001/XMLSchema#nonNegativeInteger">1</owl:qualifiedCardinality>
                <owl:onClass rdf:resource="http://www.ontologydesignpatterns.org/ont/dul/DUL.owl#Task"/>
            </owl:Restriction>
        </rdfs:subClassOf>
        <rdfs:subClassOf>
            <owl:Restriction>
                <owl:onProperty rdf:resource="http://www.ease-crc.org/ont/EASE-WF.owl#hasSuccessorTask"/>
                <owl:qualifiedCardinality rdf:datatype="http://www.w3.org/2001/XMLSchema#nonNegativeInteger">1</owl:qualifiedCardinality>
                <owl:onClass rdf:resource="http://www.ontologydesignpatterns.org/ont/dul/DUL.owl#Task"/>
            </owl:Restriction>
        </rdfs:subClassOf>
        <rdfs:comment>A relation that holds in some descriptive context such as a Workflow, between two Tasks belonging to that same Workflow. It means that one task should follow the other.

Note: a successor relation implemented as an OWL object property is sometimes enough, but not in general; in particular, when there are conditions imposed on the succession.

As a result, a reification pattern was applied here.</rdfs:comment>
        <rdfs:comment>Note: it is possible for a Succedence relation to exist between a Task and itself; in this case, both the hasPredecessorTask and hasSuccessorTask roles are filled by the same Task individual.

Care must be taken with this however, as a natural interpretation of this situation is an infinite loop.</rdfs:comment>
    </owl:Class>
    


    <!-- http://www.ontologydesignpatterns.org/ont/dul/DUL.owl#Concept -->

    <owl:Class rdf:about="http://www.ontologydesignpatterns.org/ont/dul/DUL.owl#Concept"/>
    


    <!-- http://www.ontologydesignpatterns.org/ont/dul/DUL.owl#Description -->

    <owl:Class rdf:about="http://www.ontologydesignpatterns.org/ont/dul/DUL.owl#Description"/>
    


    <!-- http://www.ontologydesignpatterns.org/ont/dul/DUL.owl#Entity -->

    <owl:Class rdf:about="http://www.ontologydesignpatterns.org/ont/dul/DUL.owl#Entity"/>
    


    <!-- http://www.ontologydesignpatterns.org/ont/dul/DUL.owl#Parameter -->

    <owl:Class rdf:about="http://www.ontologydesignpatterns.org/ont/dul/DUL.owl#Parameter"/>
    


    <!-- http://www.ontologydesignpatterns.org/ont/dul/DUL.owl#Relation -->

    <owl:Class rdf:about="http://www.ontologydesignpatterns.org/ont/dul/DUL.owl#Relation"/>
    


    <!-- http://www.ontologydesignpatterns.org/ont/dul/DUL.owl#Role -->

    <owl:Class rdf:about="http://www.ontologydesignpatterns.org/ont/dul/DUL.owl#Role"/>
    


    <!-- http://www.ontologydesignpatterns.org/ont/dul/DUL.owl#Task -->

    <owl:Class rdf:about="http://www.ontologydesignpatterns.org/ont/dul/DUL.owl#Task"/>
    


    <!-- http://www.ontologydesignpatterns.org/ont/dul/DUL.owl#Workflow -->

    <owl:Class rdf:about="http://www.ontologydesignpatterns.org/ont/dul/DUL.owl#Workflow"/>
</rdf:RDF>



<!-- Generated by the OWL API (version 4.2.8.20170104-2310) https://github.com/owlcs/owlapi -->

