<?xml version="1.0"?>
<rdf:RDF xmlns="http://www.ease-crc.org/ont/SOMA-AGENT.owl#"
     xml:base="http://www.ease-crc.org/ont/SOMA-AGENT.owl"
     xmlns:dc="http://purl.org/dc/elements/1.1/"
     xmlns:owl="http://www.w3.org/2002/07/owl#"
     xmlns:rdf="http://www.w3.org/1999/02/22-rdf-syntax-ns#"
     xmlns:xml="http://www.w3.org/XML/1998/namespace"
     xmlns:xsd="http://www.w3.org/2001/XMLSchema#"
     xmlns:SOMA="http://www.ease-crc.org/ont/SOMA.owl#"
     xmlns:rdfs="http://www.w3.org/2000/01/rdf-schema#">
    <owl:Ontology rdf:about="http://www.ease-crc.org/ont/SOMA-AGENT.owl">
        <owl:imports rdf:resource="http://www.ease-crc.org/ont/SOMA-ACT.owl"/>
        <owl:imports rdf:resource="http://www.ease-crc.org/ont/SOMA-IO.owl"/>
        <owl:imports rdf:resource="http://www.ease-crc.org/ont/SOMA-OBJ.owl"/>
        <owl:imports rdf:resource="http://www.ease-crc.org/ont/SOMA-STATE.owl"/>
        <owl:versionInfo>2.1.0</owl:versionInfo>
    </owl:Ontology>
    


    <!-- 
    ///////////////////////////////////////////////////////////////////////////////////////
    //
    // Object Properties
    //
    ///////////////////////////////////////////////////////////////////////////////////////
     -->


    


    <!-- http://www.ease-crc.org/ont/SOMA.owl#encapsulates -->


    <owl:ObjectProperty rdf:about="http://www.ease-crc.org/ont/SOMA.owl#encapsulates">
        <rdfs:subPropertyOf rdf:resource="http://www.ontologydesignpatterns.org/ont/dul/DUL.owl#associatedWith"/>
        <rdfs:domain rdf:resource="http://www.ease-crc.org/ont/SOMA.owl#OrderedElement"/>
        <rdfs:range rdf:resource="http://www.ontologydesignpatterns.org/ont/dul/DUL.owl#Entity"/>
        <rdfs:comment xml:lang="en">The relation between an Ordered element&apos; and an &apos;Entity&apos; it contains.</rdfs:comment>
        <rdfs:isDefinedBy rdf:resource="http://www.ease-crc.org/ont/SOMA-AGENT.owl"/>
        <rdfs:label xml:lang="en">encapsulates</rdfs:label>
    </owl:ObjectProperty>
    


    <!-- http://www.ease-crc.org/ont/SOMA.owl#hasPreference -->


    <owl:ObjectProperty rdf:about="http://www.ease-crc.org/ont/SOMA.owl#hasPreference">
        <rdfs:subPropertyOf rdf:resource="http://www.ontologydesignpatterns.org/ont/dul/DUL.owl#hasQuality"/>
        <owl:inverseOf rdf:resource="http://www.ease-crc.org/ont/SOMA.owl#isPreferenceOf"/>
        <rdfs:domain rdf:resource="http://www.ontologydesignpatterns.org/ont/dul/DUL.owl#Agent"/>
        <rdfs:range rdf:resource="http://www.ease-crc.org/ont/SOMA.owl#Preference"/>
        <rdfs:isDefinedBy rdf:resource="http://www.ease-crc.org/ont/SOMA-AGENT.owl"/>
        <rdfs:label xml:lang="en">Relates an agent to its preference quality.</rdfs:label>
        <rdfs:label xml:lang="en">has preference</rdfs:label>
    </owl:ObjectProperty>
    


    <!-- http://www.ease-crc.org/ont/SOMA.owl#isOrderedBy -->


    <owl:ObjectProperty rdf:about="http://www.ease-crc.org/ont/SOMA.owl#isOrderedBy">
        <rdfs:subPropertyOf rdf:resource="http://www.ontologydesignpatterns.org/ont/dul/DUL.owl#associatedWith"/>
        <owl:inverseOf rdf:resource="http://www.ease-crc.org/ont/SOMA.owl#orders"/>
        <rdfs:domain rdf:resource="http://www.ease-crc.org/ont/SOMA.owl#OrderedElement"/>
        <rdfs:range rdf:resource="http://www.ease-crc.org/ont/SOMA.owl#Order"/>
        <rdfs:comment xml:lang="en">The relation between an &apos;Order item&apos; and the &apos;Order&apos; that sorts them (via the relations &apos;precedes&apos; and &apos;follows&apos;)</rdfs:comment>
        <rdfs:isDefinedBy rdf:resource="http://www.ease-crc.org/ont/SOMA-AGENT.owl"/>
        <rdfs:label xml:lang="en">is ordered by</rdfs:label>
    </owl:ObjectProperty>
    


    <!-- http://www.ease-crc.org/ont/SOMA.owl#isPreferenceOf -->


    <owl:ObjectProperty rdf:about="http://www.ease-crc.org/ont/SOMA.owl#isPreferenceOf">
        <rdfs:subPropertyOf rdf:resource="http://www.ontologydesignpatterns.org/ont/dul/DUL.owl#isQualityOf"/>
        <rdfs:domain rdf:resource="http://www.ease-crc.org/ont/SOMA.owl#Preference"/>
        <rdfs:range rdf:resource="http://www.ontologydesignpatterns.org/ont/dul/DUL.owl#Agent"/>
        <rdfs:comment xml:lang="en">Relates a preference quality to the agent the preference belongs to.</rdfs:comment>
        <rdfs:isDefinedBy rdf:resource="http://www.ease-crc.org/ont/SOMA-AGENT.owl"/>
        <rdfs:label xml:lang="en">is preference of</rdfs:label>
    </owl:ObjectProperty>
    


    <!-- http://www.ease-crc.org/ont/SOMA.owl#orders -->


    <owl:ObjectProperty rdf:about="http://www.ease-crc.org/ont/SOMA.owl#orders">
        <rdfs:subPropertyOf rdf:resource="http://www.ontologydesignpatterns.org/ont/dul/DUL.owl#associatedWith"/>
        <rdfs:domain rdf:resource="http://www.ease-crc.org/ont/SOMA.owl#Order"/>
        <rdfs:range rdf:resource="http://www.ease-crc.org/ont/SOMA.owl#OrderedElement"/>
        <rdfs:comment xml:lang="en">The relation between an &apos;Order&apos; and the sorted &apos;Order item&apos; (sorted via the relations &apos;precedes&apos; and &apos;follows&apos; between the &apos;Order item&apos;s)</rdfs:comment>
        <rdfs:isDefinedBy rdf:resource="http://www.ease-crc.org/ont/SOMA-AGENT.owl"/>
        <rdfs:label xml:lang="en">orders</rdfs:label>
    </owl:ObjectProperty>
    


    <!-- 
    ///////////////////////////////////////////////////////////////////////////////////////
    //
    // Classes
    //
    ///////////////////////////////////////////////////////////////////////////////////////
     -->


    


    <!-- http://www.ease-crc.org/ont/SOMA.owl#AgentRole -->


    <owl:Class rdf:about="http://www.ease-crc.org/ont/SOMA.owl#AgentRole">
        <rdfs:isDefinedBy rdf:resource="http://www.ease-crc.org/ont/SOMA-AGENT.owl"/>
    </owl:Class>
    


    <!-- http://www.ease-crc.org/ont/SOMA.owl#Choice -->


    <owl:Class rdf:about="http://www.ease-crc.org/ont/SOMA.owl#Choice">
        <rdfs:subClassOf rdf:resource="http://www.ease-crc.org/ont/SOMA.owl#ResultRole"/>
        <rdfs:comment xml:lang="en">The output of a, e.g, Selecting Task.</rdfs:comment>
        <rdfs:isDefinedBy rdf:resource="http://www.ease-crc.org/ont/SOMA-AGENT.owl"/>
        <rdfs:label xml:lang="en">Choice</rdfs:label>
    </owl:Class>
    


    <!-- http://www.ease-crc.org/ont/SOMA.owl#Option -->


    <owl:Class rdf:about="http://www.ease-crc.org/ont/SOMA.owl#Option">
        <rdfs:subClassOf rdf:resource="http://www.ease-crc.org/ont/SOMA.owl#ResourceRole"/>
        <rdfs:comment xml:lang="en">The Role of objects that are used, e.g., in Selecting Tasks.</rdfs:comment>
        <rdfs:isDefinedBy rdf:resource="http://www.ease-crc.org/ont/SOMA-AGENT.owl"/>
        <rdfs:label xml:lang="en">Option</rdfs:label>
    </owl:Class>
    


    <!-- http://www.ease-crc.org/ont/SOMA.owl#Order -->


    <owl:Class rdf:about="http://www.ease-crc.org/ont/SOMA.owl#Order">
        <rdfs:subClassOf rdf:resource="http://www.ontologydesignpatterns.org/ont/dul/DUL.owl#FormalEntity"/>
        <rdfs:subClassOf>
            <owl:Restriction>
                <owl:onProperty rdf:resource="http://www.ease-crc.org/ont/SOMA.owl#orders"/>
                <owl:someValuesFrom rdf:resource="http://www.ease-crc.org/ont/SOMA.owl#OrderedElement"/>
            </owl:Restriction>
        </rdfs:subClassOf>
        <rdfs:comment xml:lang="en">An &apos;Order&apos; sorts two or more &apos;Order item&apos;s via the relations &apos;precedes&apos; and &apos;follows&apos;.</rdfs:comment>
        <rdfs:isDefinedBy rdf:resource="http://www.ease-crc.org/ont/SOMA-AGENT.owl"/>
        <rdfs:label xml:lang="en">Order</rdfs:label>
    </owl:Class>
    


    <!-- http://www.ease-crc.org/ont/SOMA.owl#OrderedElement -->


    <owl:Class rdf:about="http://www.ease-crc.org/ont/SOMA.owl#OrderedElement">
        <rdfs:subClassOf rdf:resource="http://www.ease-crc.org/ont/SOMA.owl#Singleton"/>
        <rdfs:subClassOf>
            <owl:Restriction>
                <owl:onProperty rdf:resource="http://www.ontologydesignpatterns.org/ont/dul/DUL.owl#follows"/>
                <owl:allValuesFrom rdf:resource="http://www.ease-crc.org/ont/SOMA.owl#OrderedElement"/>
            </owl:Restriction>
        </rdfs:subClassOf>
        <rdfs:subClassOf>
            <owl:Restriction>
                <owl:onProperty rdf:resource="http://www.ontologydesignpatterns.org/ont/dul/DUL.owl#precedes"/>
                <owl:allValuesFrom rdf:resource="http://www.ease-crc.org/ont/SOMA.owl#OrderedElement"/>
            </owl:Restriction>
        </rdfs:subClassOf>
        <rdfs:subClassOf>
            <owl:Restriction>
                <owl:onProperty rdf:resource="http://www.ease-crc.org/ont/SOMA.owl#isOrderedBy"/>
                <owl:qualifiedCardinality rdf:datatype="http://www.w3.org/2001/XMLSchema#nonNegativeInteger">1</owl:qualifiedCardinality>
                <owl:onClass rdf:resource="http://www.ease-crc.org/ont/SOMA.owl#Order"/>
            </owl:Restriction>
        </rdfs:subClassOf>
        <rdfs:comment xml:lang="en">A &apos;Singleton&apos; of an entity that &apos;is ordered by&apos; some &apos;Order&apos;. An &apos;Order item&apos; can only &apos;precede&apos; or &apos;follow&apos; another &apos;Order item&apos;, encoding the sortation of the entities contained within the &apos;Order items&apos;. Different &apos;Order&apos;s need to use different &apos;Order item&apos;s.</rdfs:comment>
        <rdfs:isDefinedBy rdf:resource="http://www.ease-crc.org/ont/SOMA-AGENT.owl"/>
        <rdfs:label xml:lang="en">Ordered element</rdfs:label>
    </owl:Class>
    


    <!-- http://www.ease-crc.org/ont/SOMA.owl#Predilection -->


    <owl:Class rdf:about="http://www.ease-crc.org/ont/SOMA.owl#Predilection">
        <rdfs:subClassOf rdf:resource="http://www.ontologydesignpatterns.org/ont/dul/DUL.owl#SocialRelation"/>
        <rdfs:subClassOf>
            <owl:Restriction>
                <owl:onProperty rdf:resource="http://www.ontologydesignpatterns.org/ont/dul/DUL.owl#describes"/>
                <owl:allValuesFrom>
                    <owl:Class>
                        <owl:unionOf rdf:parseType="Collection">
                            <rdf:Description rdf:about="http://www.ease-crc.org/ont/SOMA.owl#Preference"/>
                            <owl:Class>
                                <owl:intersectionOf rdf:parseType="Collection">
                                    <rdf:Description rdf:about="http://www.ease-crc.org/ont/SOMA.owl#Order"/>
                                    <owl:Restriction>
                                        <owl:onProperty rdf:resource="http://www.ease-crc.org/ont/SOMA.owl#orders"/>
                                        <owl:allValuesFrom>
                                            <owl:Restriction>
                                                <owl:onProperty rdf:resource="http://www.ease-crc.org/ont/SOMA.owl#encapsulates"/>
                                                <owl:allValuesFrom rdf:resource="http://www.ontologydesignpatterns.org/ont/dul/DUL.owl#Situation"/>
                                            </owl:Restriction>
                                        </owl:allValuesFrom>
                                    </owl:Restriction>
                                </owl:intersectionOf>
                            </owl:Class>
                        </owl:unionOf>
                    </owl:Class>
                </owl:allValuesFrom>
            </owl:Restriction>
        </rdfs:subClassOf>
        <rdfs:isDefinedBy rdf:resource="http://www.ease-crc.org/ont/SOMA-AGENT.owl"/>
        <rdfs:label xml:lang="en">The relation between a &apos;Preference&apos; and the &apos;Order&apos; that the &apos;Preference&apos; defines over Situations.

For the complete model, see &apos;Preference&apos;.</rdfs:label>
        <rdfs:label>Predilection</rdfs:label>
    </owl:Class>
    


    <!-- http://www.ease-crc.org/ont/SOMA.owl#Preference -->


    <owl:Class rdf:about="http://www.ease-crc.org/ont/SOMA.owl#Preference">
        <rdfs:subClassOf rdf:resource="http://www.ease-crc.org/ont/SOMA.owl#SocialQuality"/>
        <rdfs:subClassOf>
            <owl:Restriction>
                <owl:onProperty rdf:resource="http://www.ease-crc.org/ont/SOMA.owl#isPreferenceOf"/>
                <owl:allValuesFrom rdf:resource="http://www.ontologydesignpatterns.org/ont/dul/DUL.owl#Agent"/>
            </owl:Restriction>
        </rdfs:subClassOf>
        <rdfs:comment xml:lang="en">A &apos;Preference&apos; is a &apos;Quality&apos; of an &apos;Agent&apos; that orders &apos;Situation&apos;s by some heuristic based on the happiness, satisfaction, gratification, morality, enjoyment, and utility (see alse https://en.wikipedia.org/wiki/Preference) they provide to their bearing Agent.

The pattern is as follows: A &apos;Preference&apos; &apos;is described by&apos; a &apos;Predilection&apos;, which also &apos;describes&apos; an &apos;Order&apos; that &apos;orders&apos; &apos;Order item&apos;s that contain only &apos;Situation&apos;s. The &apos;Situation&apos;s then are modeled according to what the preference entails.

That a &apos;Preference&apos; orders &apos;Situation&apos;s might be unintuitive, but makes the model very general. A few examples:

Example 1

&quot;Peter likes coffee and dislikes tea&quot;.
Here, between different hypothetical situations where he plays the role of a performer in a drinking task, Peter prefers the situations in which role of the drunken object is played by some coffee (vs. some tea). Note that the coffe and tea are hypothetical objects as well and could, for example, be represented via reified Concepts.

Example 2

&quot;Would you like this pot of coffee, or this pot of tea, Peter?&quot;
Here, as opposed to Example 1, the pot of coffee and the pot of tea are not hypothetical, but concrete.

Example 3

&quot;Would you like this pot of coffee, or should I brew you some tea?&quot;
Here, the pot of coffee is concrete and the tea is not.

Example 4

Situations are not restricted to Tasks; other event types are possible as well.
For example, Peter might prefer the Containment State of a tiger being inside a cage vs. the Containment State of the tiger being outside of the cage.</rdfs:comment>
        <rdfs:isDefinedBy rdf:resource="http://www.ease-crc.org/ont/SOMA-AGENT.owl"/>
        <rdfs:label xml:lang="en">Preference</rdfs:label>
    </owl:Class>
    


    <!-- http://www.ease-crc.org/ont/SOMA.owl#PreferenceOrder -->


    <owl:Class rdf:about="http://www.ease-crc.org/ont/SOMA.owl#PreferenceOrder">
        <rdfs:subClassOf rdf:resource="http://www.ontologydesignpatterns.org/ont/dul/DUL.owl#SocialRelation"/>
        <rdfs:subClassOf>
            <owl:Restriction>
                <owl:onProperty rdf:resource="http://www.ease-crc.org/ont/SOMA.owl#orders"/>
                <owl:someValuesFrom rdf:resource="http://www.ease-crc.org/ont/SOMA.owl#OrderedElement"/>
            </owl:Restriction>
        </rdfs:subClassOf>
        <rdfs:subClassOf>
            <owl:Restriction>
                <owl:onProperty rdf:resource="http://www.ease-crc.org/ont/SOMA.owl#orders"/>
                <owl:allValuesFrom>
                    <owl:Restriction>
                        <owl:onProperty rdf:resource="http://www.ease-crc.org/ont/SOMA.owl#encapsulates"/>
                        <owl:allValuesFrom rdf:resource="http://www.ontologydesignpatterns.org/ont/dul/DUL.owl#Description"/>
                    </owl:Restriction>
                </owl:allValuesFrom>
            </owl:Restriction>
        </rdfs:subClassOf>
        <rdfs:subClassOf>
            <owl:Restriction>
                <owl:onProperty rdf:resource="http://www.ontologydesignpatterns.org/ont/dul/DUL.owl#describes"/>
                <owl:allValuesFrom rdf:resource="http://www.ease-crc.org/ont/SOMA.owl#Preference"/>
            </owl:Restriction>
        </rdfs:subClassOf>
        <rdfs:isDefinedBy rdf:resource="http://www.ease-crc.org/ont/SOMA-AGENT.owl"/>
        <rdfs:label xml:lang="en">The relation between a &apos;Preference&apos; and the &apos;Order&apos; that the &apos;Preference&apos; defines over Descriptions of Situations.</rdfs:label>
        <rdfs:label>Preference order</rdfs:label>
    </owl:Class>
    


    <!-- http://www.ease-crc.org/ont/SOMA.owl#PreferenceRegion -->


    <owl:Class rdf:about="http://www.ease-crc.org/ont/SOMA.owl#PreferenceRegion">
        <rdfs:subClassOf rdf:resource="http://www.ontologydesignpatterns.org/ont/dul/DUL.owl#SocialObjectAttribute"/>
        <rdfs:subClassOf>
            <owl:Restriction>
                <owl:onProperty rdf:resource="http://www.ontologydesignpatterns.org/ont/dul/DUL.owl#isRegionFor"/>
                <owl:someValuesFrom rdf:resource="http://www.ease-crc.org/ont/SOMA.owl#Preference"/>
            </owl:Restriction>
        </rdfs:subClassOf>
        <rdfs:comment xml:lang="en">The &apos;Region&apos; of &apos;Preference&apos;s, containing all possible &apos;Order&apos;s between all possible &apos;Situation&apos;s.</rdfs:comment>
        <rdfs:isDefinedBy rdf:resource="http://www.ease-crc.org/ont/SOMA-AGENT.owl"/>
        <rdfs:label xml:lang="en">Preference region</rdfs:label>
    </owl:Class>
    


    <!-- http://www.ease-crc.org/ont/SOMA.owl#Selecting -->


    <owl:Class rdf:about="http://www.ease-crc.org/ont/SOMA.owl#Selecting">
        <rdfs:subClassOf rdf:resource="http://www.ease-crc.org/ont/SOMA.owl#Deciding"/>
        <rdfs:comment xml:lang="en">A Task where an Agent decides between two or more options.</rdfs:comment>
        <rdfs:isDefinedBy rdf:resource="http://www.ease-crc.org/ont/SOMA-AGENT.owl"/>
        <rdfs:label xml:lang="en">Selecting</rdfs:label>
    </owl:Class>
    


    <!-- http://www.ease-crc.org/ont/SOMA.owl#Singleton -->


    <owl:Class rdf:about="http://www.ease-crc.org/ont/SOMA.owl#Singleton">
        <owl:equivalentClass>
            <owl:Class>
                <owl:intersectionOf rdf:parseType="Collection">
                    <rdf:Description rdf:about="http://www.ontologydesignpatterns.org/ont/dul/DUL.owl#Set"/>
                    <owl:Restriction>
                        <owl:onProperty rdf:resource="http://www.ease-crc.org/ont/SOMA.owl#encapsulates"/>
                        <owl:qualifiedCardinality rdf:datatype="http://www.w3.org/2001/XMLSchema#nonNegativeInteger">1</owl:qualifiedCardinality>
                        <owl:onClass rdf:resource="http://www.ontologydesignpatterns.org/ont/dul/DUL.owl#Entity"/>
                    </owl:Restriction>
                </owl:intersectionOf>
            </owl:Class>
        </owl:equivalentClass>
        <rdfs:comment>A &apos;Set&apos; that contains exactly one member.</rdfs:comment>
        <rdfs:isDefinedBy rdf:resource="http://www.ease-crc.org/ont/SOMA-AGENT.owl"/>
    </owl:Class>
</rdf:RDF>



<!-- Generated by the OWL API (version 5.1.20.2022-02-19T16:38:31Z) https://github.com/owlcs/owlapi/ -->


